CTM.v
@@ -1,0 +1,158 @@
+Require Import FunInd.
+Require Import Arith.
+Require Import List.
+Import ListNotations.
+
+Require Import TPPMark2019.Value.
+Require Import TPPMark2019.Tape.
+
+Set Implicit Arguments.
+
+Module CTM.
+  Inductive Move := MoveL | MoveR.
+  Section CTM.
+    Variable V : Type.
+    Context `{Value.class V}.
+    Variable State : Type.
+    Context `{Finite.class State}.
+    Variable T : Type.
+    Context `{Tape.class T V}.
+    
+    Record Machine :=
+      {
+        init_state : State;
+        transition : State -> V -> (V * Move * option State);
+        
+      }.
+
+    Record TMState :=
+      {
+        tape : T;
+        state : option State;
+      }.
+
+    Definition start (machine : Machine) (tape : T) : TMState :=
+      {|
+        tape := tape;
+        state := Some (init_state machine);
+      |}.
+    
+
+    Definition step (machine : Machine) (tms : TMState) : TMState :=
+      let '{|tape:=tape; state:=state|} := tms in
+      match state with
+      | None => tms
+      | Some state =>
+        let '(v, m, s) := transition machine state (Tape.read tape) in
+        let tape := Tape.write v tape in
+        let tape :=
+            match m with
+            | MoveL => Tape.move_left tape
+            | MoveR => Tape.move_right tape
+            end in
+        {| tape := tape; state := s |}
+      end.
+    Functional Scheme step_ind := Induction for step Sort Prop.
+
+    Lemma step_tape_size : forall machine tms,
+        Tape.size (tape tms) <> 0 ->
+        Tape.size (tape (step machine tms)) = Tape.size (tape tms).
+    Proof.
+      intros.
+      destruct tms as [tape state].
+      simpl in *.
+      destruct state; simpl; auto.
+      destruct transition as [[v m] state].
+      destruct m; simpl.
+      - rewrite !Tape.to_list_size.
+        rewrite Tape.move_left_list.
+        rewrite <- !Tape.to_list_size.
+        now apply Tape.write_size.
+      - rewrite !Tape.to_list_size.
+        rewrite Tape.move_right_list.
+        rewrite <- !Tape.to_list_size.
+        now apply Tape.write_size.
+    Qed.
+    
+    
+    Fixpoint steps (n : nat) (machine : Machine) (tms : TMState) : TMState :=
+      match n with
+      | O => tms
+      | S n' => steps n' machine (step machine tms)
+      end.
+
+    Lemma steps_1 : forall machine tms, steps 1 machine tms = step machine tms.
+    Proof.
+      reflexivity.
+    Qed.
+
+    Lemma steps_add : forall n m machine tms,
+        steps n machine (steps m machine tms) = steps (n + m) machine tms.
+    Proof.
+      induction m; intros.
+      - rewrite Nat.add_0_r.
+        reflexivity.
+      - rewrite Nat.add_succ_r.
+        simpl.
+        auto.
+    Qed.
+
+    Definition Steps n machine tms tms' := steps n machine tms = tms'.
+
+    Inductive Halts : Machine -> TMState -> Prop :=
+    | halts_halted : forall machine tms, state tms = None -> Halts machine tms
+    | halts_step : forall machine tms, Halts machine (step machine tms) -> Halts machine tms.
+
+    Lemma Halts_steps : forall machine tms,
+        Halts machine tms <->
+        exists n, state (steps n machine tms) = None.
+    Proof.
+      split; intro HH.
+      - induction HH.
+        + exists 0.
+          auto.
+        + destruct IHHH as (n & IHHH).
+          exists (S n).
+          auto.
+      - destruct HH as (n & HH).
+        revert tms HH.
+        induction n; simpl.
+        + apply halts_halted. 
+        + auto using halts_step.
+    Qed.
+
+    Definition HaltWith machine tape tape' :=
+      exists n, steps n machine (start machine tape) = {| state := None; tape := tape' |}.
+
+    Lemma HaltWith_Halts : forall machine tape_init, (exists tape', HaltWith machine tape_init tape') <-> Halts machine (start machine tape_init).
+    Proof.
+      intros machine tape_init.
+      split; intro HH.
+      - destruct HH as (tms & n & Heq).
+        rewrite Halts_steps.
+        exists n.
+        rewrite Heq.
+        reflexivity.
+      - rewrite Halts_steps in HH.
+        destruct HH as [n Heq].
+        exists (tape (steps n machine (start machine tape_init))).
+        unfold HaltWith.
+        exists n.
+        destruct (steps n machine (start machine tape_init)).
+        simpl in *.
+        congruence.
+    Qed.
+
+
+    Fixpoint steps_history n machine tms :=
+      match n with
+      | O => [tms]
+      | S n' =>
+        match state tms with
+        | None => [tms]
+        | _ => tms :: steps_history n' machine (step machine tms)
+        end
+      end.
+    
+  End CTM.
+End CTM.
