Example.v
@@ -1,0 +1,208 @@
+Require Import Arith Lia.
+Require Import List.
+Import ListNotations.
+
+Require Import TPPMark2019.Value.
+Require Import TPPMark2019.Tape.
+Require Import TPPMark2019.CTM.
+Require Import TPPMark2019.Clearer.
+
+Set Implicit Arguments.
+
+Instance BoolFinite : Finite.class bool :=
+  {|
+    Finite.card := 2;
+    Finite.surj n := n =? 1;
+  |}.
+Proof.
+  destruct x; eauto.
+Defined.
+
+Instance BoolValue : @Value.class bool BoolFinite :=
+  {|
+    Value.zero := false;
+    Value.one := true;
+  |}.
+Proof.
+  - decide equality.
+  - auto.
+Defined.
+
+
+Module FunTape.
+  Record t (V : Type): Type :=
+    {
+      size: nat;
+      head: nat;
+      vs: nat -> V
+    }.
+
+  Arguments size {V} t.
+  Arguments head {V} t.
+  Arguments vs {V} t.
+  
+  Definition modh {V} (tape : t V) : nat := (head tape) mod (size tape).
+
+  Definition read {V} (tape : t V): V :=
+    vs tape (modh tape).
+  Definition write {V} (v : V) (tape : t V) : t V :=
+    {|
+      size := size tape;
+      head := head tape;
+      vs := fun i =>
+             let i := i mod size tape in
+             if Nat.eq_dec i (modh tape)
+             then v
+             else vs tape i
+    |}.
+  Definition move_right {V} (tape : t V) : t V :=
+    {|
+      size := size tape;
+      head := S (head tape) mod (size tape);
+      vs := vs tape
+    |}.
+  Definition move_left {V} (tape : t V) : t V :=
+    {|
+      size := size tape;
+      head :=
+        match head tape with
+        | 0 => size tape - 1
+        | S h => h
+        end;
+      vs := vs tape
+    |}.
+
+  Definition from_list {V} `{Value.class V}  (l : list V) : t V :=
+    {|
+      size := List.length l;
+      head := 0;
+      vs := fun i => nth i l Value.zero
+    |}.
+
+  Definition to_list {V} `{Value.class V} (tape : t V) : list V :=
+    map (vs tape) (seq 0 (size tape)).
+  Transparent to_list.
+End FunTape.
+
+Lemma map_nth_in_range {A B} (f : A -> B) xs n da db:
+  n < length xs ->
+  nth n (map f xs) db = f (nth n xs da).
+Proof.
+  intro H.
+  rewrite nth_indep with (d' := f da).
+  - apply map_nth.
+  - now rewrite map_length.
+Qed.
+
+Lemma nth_error_nth {A} : forall (l : list A) i d, i < length l -> nth_error l i = Some (nth i l d).
+Proof.
+  induction l; intros.
+  - inversion H.
+  - destruct i; simpl in *; auto.
+    apply IHl.
+    auto with arith.
+Qed.
+
+Lemma nth_error_Some_nth {A} : forall (l : list A) i x d, nth_error l i = Some x -> x = nth i l d.
+Proof.
+  induction l; intros.
+  - destruct i; discriminate.
+  - destruct i; simpl in *; auto.
+    congruence.
+Qed.
+
+Instance FunTape_Tape V `{Value.class V} : Tape.class (FunTape.t V) V :=
+  {|
+    Tape.size := FunTape.size;
+    Tape.head := fun t => FunTape.head t mod FunTape.size t;
+    Tape.read := FunTape.read;
+    Tape.write := FunTape.write;
+    Tape.move_right := FunTape.move_right;
+    Tape.move_left := FunTape.move_left;
+    Tape.to_list := FunTape.to_list;
+  |}.
+Proof.
+  all: intros.
+  all: simpl.
+  all: unfold FunTape.to_list.
+  all:auto.
+  - destruct t; simpl.
+    now rewrite map_length, seq_length.
+  - destruct t; simpl in *.
+    unfold FunTape.modh; simpl.
+    apply map_nth_error.
+    rewrite nth_error_nth with (d := 0).
+    + rewrite seq_nth; auto.
+    + rewrite seq_length; auto.
+  - destruct t.
+    simpl in *.
+    rewrite nth_error_nth with (d := v).
+    + rewrite map_nth_in_range with (da := 0).
+      * destruct Nat.eq_dec; auto.
+        unfold FunTape.modh in *.
+        simpl in *.
+        rewrite seq_nth in *; auto.
+        simpl in *.
+        rewrite Nat.mod_mod in *; auto.
+        congruence.
+      * rewrite seq_length.
+        auto.
+    + rewrite map_length, seq_length.
+      auto.
+  - destruct t. simpl in *.
+    destruct (Nat.ltb_spec i size) as [Hlt | Hge].
+    + rewrite !nth_error_nth with (d := v).
+      * rewrite !map_nth_in_range with (da := 0); try rewrite seq_length; auto.
+        rewrite seq_nth; simpl; auto.
+        rewrite Nat.mod_small; auto.
+        unfold FunTape.modh.
+        simpl.
+        destruct Nat.eq_dec; auto.
+        congruence.
+      * now rewrite map_length, seq_length.
+      * now rewrite map_length, seq_length.
+    + rewrite !(proj2 (nth_error_None _ _)); auto.
+      * now rewrite map_length, seq_length.
+      * now rewrite map_length, seq_length.
+  - destruct t.
+    simpl in *.
+    rewrite Nat.mod_mod; auto.
+    replace (S (head mod size)) with (1 + head mod size); auto.
+    rewrite Nat.add_mod; auto.
+    rewrite Nat.mod_mod; auto.
+    rewrite <- Nat.add_mod; auto.
+  - destruct t; auto; simpl in *.
+    destruct head.
+    + rewrite Nat.mod_0_l; auto.
+      rewrite Nat.mod_small; auto.
+      lia.
+    + remember (S head mod size) as x eqn: Heqx.
+      replace (S head) with (1 + head) in Heqx; auto.
+      rewrite Nat.add_mod in Heqx; auto.
+      destruct x.
+      * destruct (Nat.eq_dec size 1); subst; auto.
+        rewrite Nat.mod_1_l in *; auto with zarith.
+        destruct (Nat.eq_dec (1 + head mod size) size); try lia.
+        rewrite Nat.mod_small in Heqx; try lia.
+        cut (head mod size < size); auto with zarith.
+      * assert (1 < size) as Hgt. {
+          destruct (Nat.eq_dec size 1); try lia.
+          subst.
+          discriminate.
+        }
+        rewrite Nat.mod_1_l in Heqx; auto.
+        simpl in *.
+        rewrite Nat.mod_small in Heqx; try lia.
+        destruct (Nat.eq_dec (S (head mod size)) size) as [Heq | Hne].
+        -- rewrite Heq in *.
+           rewrite Nat.mod_same in Heqx; lia.
+        -- cut (head mod size < size); auto with zarith.
+Defined.
+
+
+Definition bool_funtape := FunTape.t bool.
+Definition example_tape : bool_funtape := FunTape.from_list [true; false; false; true; false; true; true].
+Definition clearer := Clearer.clearer (V:= bool).
+Definition history := CTM.steps_history 100 clearer (CTM.start clearer example_tape).
+Definition history_list := map (fun tms =>  (Tape.to_list (CTM.tape tms), Tape.head (CTM.tape tms), CTM.state tms)) history.
+Compute history_list.
