Tape.v
@@ -1,0 +1,264 @@
+Require Import List Arith Lia.
+Require Import TPPMark2019.Util.
+
+Set Implicit Arguments.
+
+Lemma nth_error_eq {A} : forall (xs ys : list A), (forall i, nth_error xs i = nth_error ys i) <-> xs = ys.
+Proof.
+  intros.
+  split; intros; subst; auto.
+  revert ys H.
+  induction xs.
+  - destruct ys; auto.
+    intro H.
+    specialize (H 0).
+    inversion H.
+  - destruct ys.
+    + intro H.
+      specialize (H 0).
+      inversion H.
+    + intro H.
+      f_equal.
+      * specialize (H 0).
+        now inversion H.
+      * apply IHxs.
+        intro i.
+        specialize (H (S i)).
+        apply H.
+Qed.
+
+Module Tape.
+  Class class (A : Type) (V : Type) :=
+    {
+      size: A -> nat;
+      head : A -> nat;
+      read : A -> V;
+      write : V -> A -> A;
+      move_right : A -> A;
+      move_left : A -> A;
+
+      to_list : A -> list V;
+      to_list_size : forall t, size t = length (to_list t);
+      head_spec : forall t, size t <> 0 -> head t < size t;
+      read_spec : forall t, size t <> 0 -> List.nth_error (to_list t) (head t) = Some (read t);
+      write_spec_head : forall v t, size t <> 0 -> List.nth_error (to_list (write v t)) (head t) = Some v;
+      write_spec_other : forall i v t,
+          size t <> 0 ->
+          i <> head t ->
+          List.nth_error (to_list (write v t)) i = List.nth_error (to_list t) i;
+      write_head : forall v t, head (write v t) = head t;
+      move_right_list : forall t, to_list (move_right t) = to_list t;
+      move_right_head : forall t, size t <> 0 -> head (move_right t) = S (head t) mod size t;
+      move_left_list : forall t, to_list (move_left t) = to_list t;
+      move_left_head : forall t, size t <> 0 -> head (move_left t) =
+                            match head t with
+                            | 0 => size t - 1
+                            | S h => h
+                            end
+    }.
+
+  Lemma write_spec : forall A V `{class A V} (tape : A) v i,
+      size tape <> 0 ->
+      List.nth_error (to_list (write v tape)) i =
+      if i =? head tape
+      then (Some v)
+      else List.nth_error (to_list tape) i.
+  Proof.
+    intros.
+    destruct (Nat.eqb_spec i (head tape)); subst.
+    - apply write_spec_head; auto.
+    - apply write_spec_other; auto.
+  Qed.
+  
+  Lemma write_size : forall A V `{class A V} (tape : A) (v : V),
+      size tape <> 0 -> 
+      size (write v tape) = size tape.
+  Proof.
+    intros until v.
+    intro Hnz.
+    enough (forall i, Nat.ltb i (size (write v tape)) = Nat.ltb i (size tape)) as Hltbeq.
+    - revert Hltbeq.
+      generalize (size (write v tape)) as n.
+      generalize (size tape) as m.
+      intros.
+      apply Nat.le_antisymm.
+      + specialize (Hltbeq m).
+        rewrite Nat.ltb_irrefl in Hltbeq.
+        now rewrite Nat.ltb_ge in Hltbeq.
+      + specialize (Hltbeq n).
+        rewrite Nat.ltb_irrefl in Hltbeq.
+        symmetry in Hltbeq.
+        now rewrite Nat.ltb_ge in Hltbeq.
+    - intro i.
+      destruct (List.nth_error (to_list (write v tape)) i) eqn: Heq.
+      + replace (i <? size (write v tape)) with true; symmetry; rewrite Nat.ltb_lt.
+        * destruct (Nat.eq_dec i (head tape)); subst; auto using head_spec.
+          rewrite to_list_size, <- nth_error_Some.
+          rewrite write_spec_other in Heq; congruence.
+        * rewrite to_list_size, <- nth_error_Some.
+          congruence.
+      + replace (i <? size (write v tape)) with false; symmetry;
+          rewrite Nat.ltb_ge, to_list_size, <- nth_error_None; auto.
+        destruct (Nat.eq_dec i (head tape)).
+        * subst. rewrite write_spec_head in Heq; congruence.
+        * rewrite write_spec_other in Heq; congruence.
+  Qed.
+
+  
+  Lemma move_left_size : forall A V `{class A V} (tape : A),
+      size (move_left tape) = size tape.
+  Proof.
+    intros.
+    now rewrite !to_list_size, move_left_list.
+  Qed.
+
+  Lemma move_right_size : forall A V `{class A V} (tape : A),
+      size (move_right tape) = size tape.
+  Proof.
+    intros.
+    now rewrite !to_list_size, move_right_list.
+  Qed.
+
+  Lemma read_write_id : forall A V `{class A V} (tape  : A) (v : V),
+      size tape <> 0 ->
+      v = read tape ->
+      to_list (write v tape) = to_list tape.
+  Proof.
+    intros.
+    apply nth_error_eq.
+    intro i.
+    rewrite write_spec; auto.
+    destruct_cmpbs.
+    pose proof (read_spec tape) as Hread.
+    subst.
+    intuition.
+  Qed.
+
+  Definition replace_at {A} i (xs ys : list A) (v : A) :=
+    exists a l r, length l = i /\ xs = l ++ a :: r /\ ys = l ++ v :: r.
+
+  Lemma skipn_Sn : forall {A} i (xs : list A) (x : A), nth_error xs i = Some x -> skipn i xs = x :: skipn (S i) xs.
+  Proof.
+    intros A i xs x.
+    revert i.
+    induction xs; simpl.
+    - destruct i; inversion 1.
+    - destruct i; simpl in *; try congruence.
+      apply IHxs.
+  Qed.
+
+  Lemma skipn_nth_error :
+    forall {A} s i (xs : list A), nth_error (skipn s xs) i = nth_error xs (s + i).
+  Proof.
+    induction s; intros.
+    - reflexivity.
+    - destruct xs; simpl; auto.
+      destruct i; auto.
+  Qed.
+
+  Lemma firstn_nth_error :
+    forall {A} s i (xs : list A),
+      nth_error (firstn s xs) i =
+      if i <? s
+      then nth_error xs i
+      else None.
+  Proof.
+    induction s; intros.
+    - destruct (Nat.ltb_spec i 0); simpl; try lia.
+      destruct i; auto.
+    - destruct i.
+      + destruct_cmpbs; try lia.
+        destruct xs; auto.
+      + destruct xs; simpl.
+        * destruct Nat.ltb; auto.
+        * rewrite IHs.
+          destruct_cmpbs; auto with zarith; lia.
+  Qed.
+             
+  
+  Lemma write_replace_at : forall A V `{class A V} (tape : A) (v : V),
+      size tape <> 0 ->
+      replace_at (Tape.head tape) (Tape.to_list tape) (Tape.to_list (Tape.write v tape)) v.
+  Proof.
+    intros until v.
+    intro Hsnz.
+    exists (read tape).
+    exists (List.firstn (head tape) (to_list tape)).
+    exists (List.skipn (S (head tape)) (to_list tape)).
+    pose proof (head_spec tape Hsnz) as Hhead.
+    pose Hsnz as Hlennz.
+    rewrite to_list_size in Hhead, Hlennz.
+    split; [| split].
+    - rewrite firstn_length_le; auto with zarith.
+    - rewrite <- (firstn_skipn (head tape) (to_list tape)) at 1.
+      rewrite <- skipn_Sn; auto.
+      now apply read_spec.
+    - rewrite <- (firstn_skipn (head tape) (to_list (write v tape))).
+      replace (firstn (head tape) (to_list tape)) with (firstn (head tape) (to_list (write v tape))).
+      + replace (skipn (S (head tape)) (to_list tape)) with (skipn (S (head tape)) (to_list (write v tape))).
+        * rewrite <- skipn_Sn; auto.
+          now apply write_spec_head.
+        * apply nth_error_eq.
+          intro i.
+          rewrite !skipn_nth_error.
+          apply write_spec_other; auto with zarith.
+      + apply nth_error_eq.
+        intro i.
+        rewrite !firstn_nth_error.
+        destruct_cmpb; auto.
+        apply write_spec_other; auto with zarith.
+  Qed.
+
+  Lemma count_occ_app : forall {A} eq_dec xs ys (v : A),
+      List.count_occ eq_dec (xs ++ ys) v = List.count_occ eq_dec xs v + List.count_occ eq_dec ys v.
+  Proof.
+    intros.
+    induction xs; simpl; auto.
+    destruct eq_dec; simpl; auto.
+  Qed.
+
+  Lemma write_count_occ_ge : forall A V `{class A V} (eq_dec : forall x y, {x = y} + {x <> y}) (tape : A) (v : V),
+      size tape <> 0 ->
+      List.count_occ eq_dec (to_list tape) v <=
+      List.count_occ eq_dec (to_list (Tape.write v tape)) v.
+  Proof.
+    intros.
+    cut (forall i (xs ys : list V),
+            replace_at i xs ys v -> List.count_occ eq_dec xs v <= List.count_occ eq_dec ys v).
+    - intro H'.
+      apply (H'(head tape)); auto using write_replace_at.
+    - intros i xs ys Hrep.
+      destruct Hrep as (a & l & r & Hlen & Hl & Hr).
+      subst.
+      rewrite !count_occ_app.
+      simpl.
+      repeat destruct eq_dec; subst; try congruence; auto with arith.
+  Qed.
+    
+  Lemma write_count_occ_gt : forall A V `{class A V} (eq_dec : forall x y, {x = y} + {x <> y}) (tape : A) (v : V),
+      size tape <> 0 ->
+      read tape <> v ->
+      List.count_occ eq_dec (to_list tape) v <
+      List.count_occ eq_dec (to_list (write v tape)) v.
+  Proof.
+    intros.
+    cut (forall i (xs ys : list V),
+            nth_error xs i <> Some v ->
+            replace_at i xs ys v -> List.count_occ eq_dec xs v < List.count_occ eq_dec ys v).
+    - intro H'.
+      apply (H'(head tape)); auto using write_replace_at.
+      pose proof (read_spec tape) as Hread.
+      cut_hyp Hread; auto.
+      congruence.
+    - intros i xs ys Hne Hrep.
+      destruct Hrep as (a & l & r & Hlen & Hl & Hr).
+      subst.
+      rewrite !count_occ_app.
+      simpl.
+      repeat destruct eq_dec; subst; try congruence; auto with arith.
+      contradict Hne.
+      rewrite nth_error_app2; auto.
+      rewrite Nat.sub_diag.
+      reflexivity.
+  Qed.
+End Tape.
