Util.v
@@ -1,0 +1,20 @@
+Require Import Arith.
+Require Import List.
+
+Arguments nth_error A l n : simpl nomatch.
+Ltac cut_hyp H := lapply H; [clear H; intro H|].
+
+Ltac destruct_cmpb_in_prop P := match P with
+           | context A [?p <=? ?q]  => destruct (Nat.leb_spec p q)
+           | context A [?p <? ?q]  => destruct (Nat.ltb_spec p q)
+           | context A [?p =? ?q]  => destruct (Nat.eqb_spec p q)
+           end.
+  
+Ltac destruct_cmpb :=
+  match goal with
+  | |- ?G => destruct_cmpb_in_prop G
+  | H : ?P |- _ => destruct_cmpb_in_prop P
+  end.
+
+Ltac destruct_cmpbs := repeat destruct_cmpb; auto with zarith.
+Hint Resolve Nat.mod_upper_bound.
