Value.v
@@ -1,0 +1,20 @@
+Set Implicit Arguments.
+
+Module Finite.
+  Class class (A : Type) :=
+    {
+      card : nat;
+      surj : nat -> A;
+      surj_spec : forall (x : A), exists i, i < card /\ surj i = x;
+  
+    }.
+End Finite.
+Module Value.
+  Class class (A : Type) `{Finite.class A} :=
+    {
+      eq_dec : forall (x y : A), {x = y} + {x <> y};
+      zero : A;
+      one : A;
+      zero_ne_one : zero <> one;
+    }.
+End Value.
